Add Digest primitives

src/Crypto/Digest.dfy
@@ -4,16 +4,36 @@
 include "../StandardLibrary/StandardLibrary.dfy"
 include "../StandardLibrary/UInt.dfy"
 
-module {:extern "Digest"} Digest {
+module Digest {
   import opened StandardLibrary
   import opened UInt = StandardLibrary.UInt
+  import DigestAlgo
+  import ExternDigest
 
-  datatype Algorithm = SHA_512
-
-  function method Length(alg: Algorithm): nat {
+  function method Length(alg: DigestAlgo.Algorithm): nat {
     match alg
     case SHA_512 => 64
   }
 
-  method {:extern "Digest.SHA", "Digest"} Digest(alg: Algorithm, msg: seq<uint8>) returns (digest: Result<seq<uint8>>)
+  method Digest(alg: DigestAlgo.Algorithm, msg: seq<uint8>) returns (res: Result<seq<uint8>>)
+    ensures res.Success? ==> |res.value| == Length(alg)
+  {
+    var digest := ExternDigest.Digest(alg, msg);
+    if |digest| == Length(alg) {
+        return Success(digest);
+    } else {
+        return Failure("Incorrect length digest from ExternDigest.");
+    }
+  }
+}
+
+module DigestAlgo {
+  datatype Algorithm = SHA_512
+}
+
+module {:extern "ExternDigest" } ExternDigest {
+  import opened UInt = StandardLibrary.UInt
+  import opened DigestAlgo = DigestAlgo
+
+  method {:extern } Digest(alg: DigestAlgo.Algorithm, msg: seq<uint8>) returns (digest: seq<uint8>)
 }
